MonadClass/MonadAlt.v
@@ -7,7 +7,7 @@ Class MonadAlt (M : Type -> Type) (inst : Monad M) : Type :=
     choose_assoc :
       forall {X : Type} (a b c : M X),
         choose (choose a b) c = choose a (choose b c);
-    choose_bind :
+    choose_bind_l :
       forall (A B : Type) (x y : M A) (f : A -> M B),
         choose x y >>= f = choose (x >>= f) (y >>= f);
 }.
