MonadClass/All.v
@@ -1,5 +1,10 @@
-Require Export MonadClass.MonadSkip.
+Require Export MonadClass.MonadAlt.
+Require Export MonadClass.MonadAlt2.
+Require Export MonadClass.MonadAltSet.
+Require Export MonadClass.MonadAltBag.
 Require Export MonadClass.MonadFail.
-Require Export MonadClass.MonadReader.
-Require Export MonadClass.MonadState.
 Require Export MonadClass.MonadFree.
+Require Export MonadClass.MonadNondet.
+Require Export MonadClass.MonadReader.
+Require Export MonadClass.MonadSkip.
+Require Export MonadClass.MonadState.
